Some progress on refactoring. Checkpointing to try some changes.

CrIdentifiers.v
@@ -9,12 +9,56 @@ Import ListNotations.
 
 (* Define the different types of identifiers in the Caracara DSL *)
 Inductive ParserState : Type := ParserStateCtr (uid : positive).
-Inductive Header : Type := HeaderCtr (uid : positive).
-Inductive State : Type := StateCtr (uid : positive).
 Inductive ModuleName : Type := ModuleNameCtr (uid : positive).
 Inductive FunctionName : Type := FunctionNameCtr (uid : positive).
 Inductive ConnectionName : Type := ConnectionNameCtr (uid : positive).
-Inductive Ctrl : Type := CtrlCtr (uid : positive).
+
+(* Unified CrVar that represents Header / State / Ctrl identifiers *)
+Inductive CrVar : Type :=
+| CrHdr  (uid : positive)
+| CrState (uid : positive)
+| CrCtrl  (uid : positive).
+
+(* Projection to the underlying uid *)
+Definition crvar_id (v: CrVar) : positive :=
+  match v with
+  | CrHdr uid => uid
+  | CrState uid => uid
+  | CrCtrl uid => uid
+  end.
+
+(* Kind predicates (bools are convenient for decisions and proofs) *)
+Definition is_header (v: CrVar) : bool :=
+  match v with CrHdr _ => true | _ => false end.
+Definition is_state (v: CrVar) : bool :=
+  match v with CrState _ => true | _ => false end.
+Definition is_ctrl (v: CrVar) : bool :=
+  match v with CrCtrl _ => true | _ => false end.
+
+(* Wrapper records that carry the invariant that the CrVar is of the expected kind.
+   Keeping the old names (Header / State / Ctrl) lets other modules remain largely unchanged. *)
+Record Header := mkHeader { hdr_var : CrVar; hdr_ok : is_header hdr_var = true }.
+Record State  := mkState  { st_var  : CrVar; st_ok  : is_state st_var = true }.
+Record Ctrl   := mkCtrl   { ctrl_var : CrVar; ctrl_ok : is_ctrl ctrl_var = true }.
+
+(* Coercions allow a Header/State/Ctrl to be used where CrVar is expected *)
+Coercion hdr_var : Header >-> CrVar.
+Coercion st_var  : State  >-> CrVar.
+Coercion ctrl_var: Ctrl   >-> CrVar.
+
+(* Smart constructors for easy construction where the underlying invariant is evident *)
+Definition make_header (uid : positive) : Header := mkHeader (CrHdr uid) eq_refl.
+Definition make_state  (uid : positive) : State  := mkState  (CrState uid) eq_refl.
+Definition make_ctrl   (uid : positive) : Ctrl   := mkCtrl   (CrCtrl uid) eq_refl.
+
+(* Convenience equality test on CrVar by id and constructor tag *)
+Definition crvar_eqb (a b : CrVar) : bool :=
+  match a, b with
+  | CrHdr sa,   CrHdr sb   => Pos.eqb sa sb
+  | CrState sa, CrState sb => Pos.eqb sa sb
+  | CrCtrl sa,  CrCtrl sb  => Pos.eqb sa sb
+  | _, _ => false
+  end.
 
 (* Equality check functions for the identifiers above *)
 Definition parser_state_equal (p1 p2 : ParserState) :=
@@ -26,17 +70,14 @@ Definition parser_state_equal' (p1 p2 : ParserState) :=
         match p1, p2 with
         | ParserStateCtr xid, ParserStateCtr yid => Pos.eqb xid yid
         end.
+
 (* Do the same thing as parser_state_equal for Header *)
 Definition header_equal (h1 h2 : Header) :=
-    match h1, h2 with
-            | HeaderCtr xid, HeaderCtr yid => Pos.eqb xid yid
-    end.
+    crvar_eqb h1 h2.
 
 (* Do the same thing as parser_state_equal for State *)
 Definition state_equal (sv1 sv2 : State) :=
-    match sv1, sv2 with
-            | StateCtr xid, StateCtr yid => Pos.eqb xid yid
-    end.
+    crvar_eqb sv1 sv2.
 
 (* Do the same thing as parser_state_equal for ModuleName *)
 Definition module_name_equal (m1 m2 : ModuleName) :=
@@ -58,18 +99,19 @@ Definition connection_name_equal (c1 c2 : ConnectionName) :=
 
 (* Do the same thing as parser_state_equal for Ctrl *)
 Definition ctrl_equal (cc1 cc2 : Ctrl) :=
-    match cc1, cc2 with
-            | CtrlCtr xid, CtrlCtr yid => Pos.eqb xid yid
-    end.
+    crvar_eqb cc1 cc2.
+
+Require Import Coq.Logic.ProofIrrelevance.
 
 Lemma header_equal_lemma :
   forall h1 h2,
   header_equal h1 h2 = true ->
   h1 = h2.
 Proof.
-  intros h1 h2 H.
-  destruct h1, h2; simpl in H; try congruence.
-  apply Pos.eqb_eq in H. subst. reflexivity.
+  intros [v1 p1] [v2 p2] H.
+  unfold header_equal, crvar_eqb in H. simpl in H.
+  destruct v1; destruct v2; simpl in H; try discriminate.
+  apply Pos.eqb_eq in H. subst. f_equal. apply proof_irrelevance.
 Qed.
 
 Fixpoint hdr_list_equal (h1 : list Header) (h2 : list Header) :=
@@ -103,7 +145,8 @@ Lemma state_equal_lemma :
 Proof.
   intros s1 s2 H.
   destruct s1, s2; simpl in H; try congruence.
-  apply Pos.eqb_eq in H. subst. reflexivity.
+  destruct st_var0, st_var1; simpl in H; try discriminate.
+  apply Pos.eqb_eq in H. subst. f_equal. apply proof_irrelevance.
 Qed.
 
 (* Do the same thing as above
@@ -145,8 +188,10 @@ Lemma ctrl_equal_lemma :
   c1 = c2.
 Proof.
   intros c1 c2 H.
-  destruct c1, c2; simpl in H; try congruence.
-  apply Pos.eqb_eq in H. subst. reflexivity.
+  destruct c1, c2; simpl in H.
+  unfold ctrl_equal, crvar_eqb in H. simpl in H.
+  destruct ctrl_var0, ctrl_var1; simpl in H; try discriminate.
+  apply Pos.eqb_eq in H. subst. f_equal. apply proof_irrelevance.
 Qed.
 
 Lemma ctrl_list_equal_lemma:
